src/program_proof/session/sort.v
@@ -383,7 +383,8 @@ Section heap.
         eapply H9; eassumption.
       + destruct H10. auto.
   Qed.
-  
+
+  (*
   Lemma wp_sortedInsert (s: Slice.t) (l: list Operation.t)
     (opv: Slice.t*u64) (v: Operation.t) (n: nat) :
     {{{
@@ -655,6 +656,7 @@ Section heap.
                 ** intros. eapply H6.
                    { assert (uint.nat w <= j') by word. apply H8. }
                    { auto. } *)
-  Admitted. 
+  Admitted.
+  *)
 
 End heap.
